src/PL/semantics.lean
@@ -11,31 +11,81 @@ structure Structure := (val : A → bool)
 
 variables {A} (S : Structure A)
 
-@[simp] def formula.val : formula A → bool
+@[simp] def formula.val : formula A → Prop
 | (atom a) := S.val a
 | ⊤        := true
-| (p ⟶ q) := bnot p.val || q.val
-| (⁻p)     := bnot p.val
+| (p ⟶ q) := p.val → q.val
+| (⁻p)     := ¬p.val
 
 instance : semantics (formula A) (Structure A) := ⟨λ S p, p.val S⟩
 
-lemma models_def (S : Structure A) (p : formula A) : S ⊧ p ↔ p.val S = tt :=
+lemma models_def (S : Structure A) (p : formula A) : S ⊧ p ↔ p.val S :=
 by refl 
 
-variables {T : theory A} {p : formula A}
+instance : has_double_turnstile (Theory A) (formula A) := ⟨semantics.consequence (Structure A)⟩
 
-lemma soundness (b : T ⊢ p) : T ⊧[Structure A] p :=
+lemma consequence_def {T : Theory A} {p : formula A} :
+  T ⊧ p ↔ semantics.consequence (Structure A) T p := by refl
+
+variables {T : Theory A} {p : formula A}
+
+lemma soundness (b : T ⊢ p) : T ⊧ p :=
 begin
   apply rec'_on b,
-  { intros p q hpq hp IHpq IHp S h, 
-    have l₁ : p.val S = ff ∨ q.val S = tt, by simpa[models_def] using IHpq h,
-    have l₂ : p.val S = tt, by simpa[models_def] using IHp h,
-    simpa[l₂, models_def] using l₁ },
+  { intros p q hpq hp IHpq IHp S h, exact (IHpq h) (IHp h) },
   { intros p hp S h, exact h hp },
   { intros S hS, simp[models_def] },
-  { intros p q S hS, simp[models_def], cases p.val S; simp },
-  { intros p q r S hS, simp[models_def], cases p.val S; cases q.val S; cases r.val S; simp },
-  { intros p q S hS, simp[models_def], cases p.val S; cases q.val S; simp }
+  { intros p q S hS h₁ h₂, exact h₁},
+  { intros p q r S hS h₁ h₂ h₃, exact h₁ h₃ (h₂ h₃) },
+  { intros p q S hS h₁ h₂, exact not_imp_not.mp h₁ h₂ }
 end
+
+instance : sound (formula A) (Structure A) := ⟨λ _ _, soundness⟩
+
+namespace Structure
+variables {S}
+
+@[simp] lemma models_verum : S ⊧ (⊤ : formula A) := by simp[models_def]
+
+@[simp] lemma models_falsum : ¬S ⊧ (⊥ : formula A) := by simp[models_def, bot_def]
+
+@[simp] lemma models_imply {p q : formula A} : S ⊧ p ⟶ q ↔ (S ⊧ p → S ⊧ q) :=
+by refl
+
+@[simp] lemma models_not {p : formula A} : S ⊧ ⁻p ↔ ¬S ⊧ p :=
+by refl
+
+end Structure
+
+namespace completeness
+open logic.Theory.consistent logic.semantics
+variables {T}
+
+noncomputable def model (T : Theory A) : Structure A := ⟨λ a, atom a ∈ maximal T⟩
+
+lemma model_models_iff (consis : T.consistent) : p ∈ maximal T ↔ model T ⊧ p :=
+begin
+  induction p,
+  case atom { simp[models_def, model] },
+  case verum { simp[models_def], refine (mem_maximal_iff consis).mpr (by simp) },
+  case imply : p q IH₁ IH₂ { simp[imply_mem_maximal_iff consis, IH₁, IH₂] },
+  case neg : p IH { simp[neg_mem_maximal_iff consis, IH] }
+end
+
+lemma model_models (consis : T.consistent) : model T ⊧ T := λ p hp,
+(model_models_iff consis).mp (ss_maximal consis hp)
+
+theorem consistent_iff_satisfiable : Theory.consistent T ↔ Satisfiable (Structure A) T :=
+⟨λ consis,  ⟨_, model_models consis⟩, by { rintros ⟨M, hM⟩, by { exact Structure_consistent (by simp) hM }}⟩
+
+theorem completeness {p : formula A} : T ⊢ p ↔ T ⊧ p :=
+⟨soundness, by {
+  simp[Theory.provable_iff_inconsistent, consistent_iff_satisfiable], rintros h ⟨S, hS⟩,
+  have l : ¬p.val S ∧ S ⊧ T, by simpa[models_def] using hS,
+  have : S ⊧ p, from h l.2,
+  have : ¬S ⊧ p, from l.1,
+  contradiction }⟩
+
+end completeness
 
 end pl
